extraction/chord/coq/ExtractChord.v
@@ -10,10 +10,10 @@ Definition SUCC_LIST_LEN := 2.
 Definition hash (a : addr) : id :=
   a mod 256.
 
-Definition handleNet : addr -> addr -> payload -> data -> res :=
+Definition handleNet : addr -> addr -> data -> payload -> res :=
   recv_handler SUCC_LIST_LEN hash.
 
-Definition init : addr -> list addr -> res :=
+Definition init : addr -> list addr -> data * list (addr * payload) * list timeout :=
   start_handler SUCC_LIST_LEN hash.
 
 Definition handleTick : addr -> data -> res :=
