systems/ChordProof.v
@@ -1,0 +1,25 @@
+Require Import DynamicNet.
+Require Import Chord.
+Require Import List.
+
+Section ChordProof.
+  Variable SUCC_LIST_LEN : nat.
+  Variable hash : addr -> id.
+  Variable hash_inj : forall a b : addr,
+      hash a = hash b -> a = b.
+
+  Notation start_handler := (start_handler SUCC_LIST_LEN hash).
+  Notation recv_handler := (recv_handler SUCC_LIST_LEN hash).
+  Notation timeout_handler := (timeout_handler hash).
+
+  Notation global_state := (global_state addr payload data timeout).
+  Notation step_dynamic := (step_dynamic addr addr_eq_dec payload data timeout timeout_eq_dec start_handler recv_handler timeout_handler client_payload can_be_client can_be_node).
+
+  Notation e_timeout := (e_timeout addr payload timeout).
+  Notation e_fail := (e_fail addr payload timeout).
+
+  Axiom timeouts_detect_failure : forall trace xs ys t h dead req,
+      t = (e_timeout h (Request dead req)) ->
+      trace = xs ++ t :: ys ->
+      In (e_fail dead) xs.
+End ChordProof.
